Bumped ITree version in cat proofs

cat/verif_cat1a.v
@@ -1,6 +1,6 @@
 Require Import VST.progs.io_specs.
 Require Import VST.floyd.proofauto.
-Require Import cat1a.
+Require Import Top.cat1a.
 
 Instance CompSpecs : compspecs. make_compspecs prog. Defined.
 Definition Vprog : varspecs. mk_varspecs prog. Defined.
@@ -9,13 +9,13 @@ Definition putchar_spec := DECLARE _putchar putchar_spec.
 Definition getchar_spec := DECLARE _getchar getchar_spec.
 
 Definition cat_loop : IO_itree :=
-   ITree.aloop (fun _ => inl (c <- read stdin;; write stdout c)) tt.
+   ITree.iter (fun _ => c <- read stdin;; write stdout c;; Ret (inl tt)) tt.
 
 Definition main_spec :=
  DECLARE _main
   WITH gv : globals
-  PRE  [] main_pre_ext prog cat_loop nil gv
-  POST [ tint ] main_post prog nil gv.
+  PRE  [] main_pre prog cat_loop gv
+  POST [ tint ] main_post prog gv.
 
 Definition Gprog : funspecs := ltac:(with_library prog [putchar_spec; getchar_spec;
   main_spec]).
@@ -23,13 +23,14 @@ Definition Gprog : funspecs := ltac:(with_library prog [putchar_spec; getchar_sp
 Lemma cat_loop_eq : cat_loop ≈ (c <- read stdin;; write stdout c;; cat_loop).
 Proof.
   intros.
-  unfold cat_loop; rewrite unfold_aloop.
-  unfold ITree._aloop.
-  rewrite tau_eutt, bind_bind.
+  unfold cat_loop; rewrite unfold_iter.
+  unfold ITree._iter.
+  rewrite bind_bind.
   apply eqit_bind; try reflexivity.
   intros [].
-  apply eqit_bind; try reflexivity.
-  intros []; reflexivity.
+  rewrite bind_bind; apply eqit_bind; try reflexivity.
+  intros [].
+  rewrite bind_ret_l; apply eqit_tauL; reflexivity.
 Qed.
 
 Lemma body_main: semax_body Vprog Gprog f_main main_spec.
@@ -70,7 +71,7 @@ Definition ext_link := ext_link_prog prog.
 Instance Espec : OracleKind := IO_Espec ext_link.
 
 Lemma prog_correct:
-  semax_prog_ext prog cat_loop Vprog Gprog.
+  semax_prog prog cat_loop Vprog Gprog.
 Proof.
 prove_semax_prog.
 semax_func_cons_ext.
